Generalize bsim

common/Smallstep.v
@@ -25,6 +25,7 @@ Require Import Coqlib.
 Require Import Events.
 Require Import Globalenvs.
 Require Import Integers.
+Require Import sflib.
 
 Set Implicit Arguments.
 
@@ -1107,9 +1108,11 @@ Record bsim_properties (L1 L2: semantics) (index: Type)
     bsim_simulation:
       forall s2 t s2', Step L2 s2 t s2' ->
       forall i s1, match_states i s1 s2 -> safe L1 s1 ->
-      exists i', exists s1',
+      (exists i', exists s1',
          (Plus L1 s1 t s1' \/ (Star L1 s1 t s1' /\ order i' i))
-      /\ match_states i' s1' s2';
+      /\ match_states i' s1' s2') \/
+      (<<PTERM: ~trace_intact t>> /\ exists s1' t',
+           <<STAR: Star L1 s1 t' s1'>> /\ <<SUB: exists tl, t' = (trace_cut_pterm t) ** tl>>);
     bsim_public_preserved:
       forall id, Senv.public_symbol (symbolenv L2) id = Senv.public_symbol (symbolenv L1) id
   }.
@@ -1131,14 +1134,14 @@ Lemma bsim_simulation':
   forall i s2 t s2', Step L2 s2 t s2' ->
   forall s1, match_states i s1 s2 -> safe L1 s1 ->
   (exists i', exists s1', Plus L1 s1 t s1' /\ match_states i' s1' s2')
-  \/ (exists i', order i' i /\ t = E0 /\ match_states i' s1 s2').
+  \/ (exists i', order i' i /\ t = E0 /\ match_states i' s1 s2') \/
+  (<<PTERM: ~trace_intact t>> /\ exists s1' t',
+       <<STAR: Star L1 s1 t' s1'>> /\ <<SUB: exists tl, t' = (trace_cut_pterm t) ** tl>>).
 Proof.
   intros. exploit bsim_simulation; eauto.
-  intros [i' [s1' [A B]]]. intuition.
-  left; exists i'; exists s1'; auto.
-  inv H4.
-  right; exists i'; auto.
-  left; exists i'; exists s1'; split; auto. econstructor; eauto.
+  i. des_safe eauto. inv H3.
+  right. left. esplits; eauto.
+  left. esplits; eauto. econs; eauto.
 Qed.
 
 (** ** Backward simulation diagrams. *)
@@ -1189,7 +1192,7 @@ Proof.
 - intros. exists tt; eauto.
 - intros. exists s1; split. apply star_refl. eauto.
 - intros. exploit simulation; eauto. intros [s1' [A B]].
-  exists tt; exists s1'; auto.
+  left. exists tt; exists s1'; auto.
 Qed.
 
 End BACKWARD_SIMULATION_PLUS.
@@ -1211,10 +1214,11 @@ Proof.
 - (* base case *)
   intros. exists i; exists s1; split; auto. apply star_refl.
 - (* inductive case *)
-  intros. exploit bsim_simulation; eauto. intros [i' [s1' [A B]]].
+  intros. exploit bsim_simulation; eauto. intros [[i' [s1' [A B]]] | PTERM].
   assert (Star L1 s0 E0 s1'). intuition. apply plus_star; auto.
   exploit H0. eauto. eapply star_safe; eauto. intros [i'' [s1'' [C D]]].
   exists i''; exists s1''; split; auto. eapply star_trans; eauto.
+  des; ss. unfold trace_intact in *. ss. (* TODO: make lemma? *)
 Qed.
 
 Lemma bsim_safe:
@@ -1234,18 +1238,20 @@ Lemma bsim_E0_plus:
 Proof.
   induction 1 using plus_ind2; intros; subst t.
 - (* base case *)
-  exploit bsim_simulation'; eauto. intros [[i' [s1' [A B]]] | [i' [A [B C]]]].
+  exploit bsim_simulation'; eauto. intros [[i' [s1' [A B]]] | [[i' [A [B C]]] | PTERM]].
 + left; exists i'; exists s1'; auto.
 + right; exists i'; intuition.
++ des. unfold trace_intact in *. ss. (* TODO: make lemma *)
 - (* inductive case *)
   exploit Eapp_E0_inv; eauto. intros [EQ1 EQ2]; subst.
-  exploit bsim_simulation'; eauto. intros [[i' [s1' [A B]]] | [i' [A [B C]]]].
+  exploit bsim_simulation'; eauto. intros [[i' [s1' [A B]]] | [[i' [A [B C]]] | PTERM]].
 + exploit bsim_E0_star. apply plus_star; eauto. eauto. eapply star_safe; eauto. apply plus_star; auto.
   intros [i'' [s1'' [P Q]]].
   left; exists i''; exists s1''; intuition. eapply plus_star_trans; eauto.
 + exploit IHplus; eauto. intros [P | [i'' [P Q]]].
   left; auto.
   right; exists i''; intuition. eapply t_trans; eauto. apply t_step; auto.
++ des. unfold trace_intact in *. ss. (* TODO: make lemma *)
 Qed.
 
 Lemma star_non_E0_split:
@@ -1296,13 +1302,15 @@ Qed.
 Lemma bb_simulation_base:
   forall s3 t s3', Step L3 s3 t s3' ->
   forall i1 s1 i2 s2, match_states i1 s1 s2 -> match_states' i2 s2 s3 -> safe L1 s1 ->
-  exists i', exists s1',
+  (exists i', exists s1',
     (Plus L1 s1 t s1' \/ (Star L1 s1 t s1' /\ bb_order i' (i1, i2)))
-    /\ bb_match_states i' s1' s3'.
+    /\ bb_match_states i' s1' s3') \/
+  (<<PTERM: ~trace_intact t>> /\ exists s1' t',
+       <<STAR: Star L1 s1 t' s1'>> /\ <<SUB: exists tl, t' = (trace_cut_pterm t) ** tl>>).
 Proof.
   intros.
   exploit (bsim_simulation' S23); eauto. eapply bsim_safe; eauto.
-  intros [ [i2' [s2' [PLUS2 MATCH2]]] | [i2' [ORD2 [EQ MATCH2]]]].
+  intros [ [i2' [s2' [PLUS2 MATCH2]]] | [[i2' [ORD2 [EQ MATCH2]]] | PTERM]].
 - (* 1 L2 makes one or several transitions *)
   assert (EITHER: t = E0 \/ (length t = 1)%nat).
   { exploit L3_single_events; eauto.
@@ -1312,8 +1320,10 @@ Proof.
   subst t. exploit (bsim_E0_plus S12); eauto.
   intros [ [i1' [s1' [PLUS1 MATCH1]]] | [i1' [ORD1 MATCH1]]].
 * (* 1.1.1 L1 makes one or several transitions *)
+  left.
   exists (i1', i2'); exists s1'; split. auto. eapply bb_match_at; eauto.
 * (* 1.1.2 L1 makes no transitions *)
+  left.
   exists (i1', i2'); exists s1; split.
   right; split. apply star_refl. left; auto.
   eapply bb_match_at; eauto.
@@ -1322,13 +1332,27 @@ Proof.
   intros [s2x [s2y [P [Q R]]]].
   exploit (bsim_E0_star S12). eexact P. eauto. auto. intros [i1' [s1x [X Y]]].
   exploit (bsim_simulation' S12). eexact Q. eauto. eapply star_safe; eauto.
-  intros [[i1'' [s1y [U V]]] | [i1'' [U [V W]]]]; try (subst t; discriminate).
+  intros [[i1'' [s1y [U V]]] | [[i1'' [U [V W]]] | PTERM]]; try (subst t; discriminate).
+  left.
   exists (i1'', i2'); exists s1y; split.
   left. eapply star_plus_trans; eauto. eapply bb_match_later; eauto.
+  { des. right. split; ss. esplits; cycle 1. { eauto. } eapply star_trans; eauto. }
 - (* 2. L2 makes no transitions *)
+  left.
   subst. exists (i1, i2'); exists s1; split.
   right; split. apply star_refl. right; auto.
   eapply bb_match_at; eauto.
+- des. right. split; ss.
+  admit "WE WILL REMOVE THIS LEMMA".
+  (* assert(exists t1 s1', Star L1 s1 t1 s1' /\ exists tl1, t1 = trace_cut_pterm t' ** tl1). *)
+  (* { clear - H2 H0 STAR S12. *)
+  (*   ginduction STAR; ii; ss. *)
+  (*   { esplits; eauto. apply star_refl. } *)
+  (*   exploit IHSTAR; eauto. *)
+  (* } *)
+  (* des. clarify. *)
+  (* esplits; eauto. *)
+  (* admit "there should be this thing". *)
 Qed.
 
 Lemma bb_simulation:
@@ -1338,27 +1362,28 @@ Lemma bb_simulation:
     (Plus L1 s1 t s1' \/ (Star L1 s1 t s1' /\ bb_order i' i))
     /\ bb_match_states i' s1' s3'.
 Proof.
-  intros. inv H0.
-  exploit star_inv; eauto. intros [[EQ1 EQ2] | PLUS].
-- (* 1. match at *)
-  subst. eapply bb_simulation_base; eauto.
-- (* 2. match later *)
-  exploit (bsim_E0_plus S12); eauto.
-  intros [[i1' [s1' [A B]]] | [i1' [A B]]].
-+ (* 2.1 one or several silent transitions *)
-  exploit bb_simulation_base. eauto. auto. eexact B. eauto.
-    eapply star_safe; eauto. eapply plus_star; eauto.
-  intros [i'' [s1'' [C D]]].
-  exists i''; exists s1''; split; auto.
-  left. eapply plus_star_trans; eauto.
-  destruct C as [P | [P Q]]. apply plus_star; eauto. eauto.
-  traceEq.
-+ (* 2.2 no silent transition *)
-  exploit bb_simulation_base. eauto. auto. eexact B. eauto. auto.
-  intros [i'' [s1'' [C D]]].
-  exists i''; exists s1''; split; auto.
-  intuition. right; intuition.
-  inv H6. left. eapply t_trans; eauto. left; auto.
+  admit "WE WILL REMOVE THIS LEMMA".
+(*   intros. inv H0. *)
+(*   exploit star_inv; eauto. intros [[EQ1 EQ2] | PLUS]. *)
+(* - (* 1. match at *) *)
+(*   subst. eapply bb_simulation_base; eauto. *)
+(* - (* 2. match later *) *)
+(*   exploit (bsim_E0_plus S12); eauto. *)
+(*   intros [[i1' [s1' [A B]]] | [i1' [A B]]]. *)
+(* + (* 2.1 one or several silent transitions *) *)
+(*   exploit bb_simulation_base. eauto. auto. eexact B. eauto. *)
+(*     eapply star_safe; eauto. eapply plus_star; eauto. *)
+(*   intros [i'' [s1'' [C D]]]. *)
+(*   exists i''; exists s1''; split; auto. *)
+(*   left. eapply plus_star_trans; eauto. *)
+(*   destruct C as [P | [P Q]]. apply plus_star; eauto. eauto. *)
+(*   traceEq. *)
+(* + (* 2.2 no silent transition *) *)
+(*   exploit bb_simulation_base. eauto. auto. eexact B. eauto. auto. *)
+(*   intros [i'' [s1'' [C D]]]. *)
+(*   exists i''; exists s1''; split; auto. *)
+(*   intuition. right; intuition. *)
+(*   inv H6. left. eapply t_trans; eauto. left; auto. *)
 Qed.
 
 End COMPOSE_BACKWARD_SIMULATIONS.
@@ -1398,7 +1423,8 @@ Proof.
   intros i s1 s3 MS SAFE. inv MS.
   eapply (bsim_progress props'). eauto. eapply star_safe; eauto. eapply bsim_safe; eauto.
 - (* simulation *)
-  apply bb_simulation; auto.
+  admit "WE WILL REMOVE THIS LEMMA".
+  (* apply bb_simulation; auto. *)
 - (* symbols *)
   intros. transitivity (Senv.public_symbol (symbolenv L2) id); eapply bsim_public_preserved; eauto.
 Qed.
@@ -1693,6 +1719,7 @@ Proof.
   inv H4. congruence. right; econstructor; econstructor; eauto.
   inv H1. right; econstructor; econstructor; eauto.
 - (* simulation *)
+  i. left.
   eapply f2b_simulation_step; eauto.
 - (* symbols preserved *)
   exact (fsim_public_preserved FS).
@@ -1839,38 +1866,76 @@ Inductive fbs_match: index -> state L1 -> (trace * state L2) -> Prop :=
   | fbs_match_intro: forall i s1 t s2 s1',
       Star L1 s1 t s1' -> match_states i s1' s2 ->
       t = E0 \/ output_trace t ->
+      fbs_match i s1 (t, s2)
+  | fbs_match_pterm_intro: forall
+      i s1 t s2 s1' (PTERM: ~trace_intact t) (WB: output_trace t)
+      (SRC: Star L1 s1 (trace_cut_pterm t) s1'),
       fbs_match i s1 (t, s2).
 
 Lemma fbs_simulation:
   forall s2 t s2', Step (atomic L2) s2 t s2' ->
   forall i s1, fbs_match i s1 s2 -> safe L1 s1 ->
-  exists i', exists s1',
+  (exists i', exists s1',
      (Plus L1 s1 t s1' \/ (Star L1 s1 t s1' /\ order i' i))
-     /\ fbs_match i' s1' s2'.
+     /\ fbs_match i' s1' s2') \/
+  (<<PTERM: ~trace_intact t>> /\ exists s1' t',
+       <<STAR: Star L1 s1 t' s1'>> /\ <<SUB: exists tl, t' = (trace_cut_pterm t) ** tl>>).
 Proof.
   induction 1; intros.
 - (* silent step *)
-  inv H0.
+  inv H0; cycle 1.
+  { unfold trace_intact in *. ss. (* TODO: make lemma *) }
   exploit (bsim_simulation sim); eauto. eapply star_safe; eauto.
-  intros [i' [s1'' [A B]]].
+  intros [[i' [s1'' [A B]]] | PTERM].
+  left.
   exists i'; exists s1''; split.
   destruct A as [P | [P Q]]. left. eapply star_plus_trans; eauto. right; split; auto. eapply star_trans; eauto.
   econstructor. apply star_refl. auto. auto.
+  { des_safe. unfold trace_intact in *. ss. (* TODO: make lemma *) }
 - (* start step *)
-  inv H0.
+  inv H0; cycle 1.
+  { unfold trace_intact in *. ss. (* TODO: make lemma *) }
   exploit (bsim_simulation sim); eauto. eapply star_safe; eauto.
-  intros [i' [s1'' [A B]]].
+  intros [[i' [s1'' [A B]]] | PTERM].
   assert (C: Star L1 s1 (ev :: t) s1'').
     eapply star_trans. eauto. destruct A as [P | [P Q]]. apply plus_star; eauto. eauto. auto.
   exploit star_non_E0_split'; eauto. simpl. intros [s1x [P Q]].
+  left.
   exists i'; exists s1x; split.
   left; auto.
   econstructor; eauto.
   exploit L2wb; eauto.
+  { des_safe.
+    destruct (Classical_Prop.classic (ev = Event_pterm)).
+    - clarify. right. split; ss. { unfold trace_intact. ii. apply H0. ss. eauto. } esplits; eauto.
+    - left. replace (trace_cut_pterm (ev :: t) ** tl) with (ev :: trace_cut_pterm (t) ** tl) in STAR; cycle 1.
+      { ss. des_ifs. }
+      apply star_non_E0_split' in STAR; ss. des_safe.
+      assert(exists s2y, Star L1 s2x (trace_cut_pterm t) s2y /\ Star L1 s2y tl s1'0).
+      { admit "ez - single events". }
+      des_safe.
+      esplits; eauto.
+      + left. eapply star_plus_trans; eauto.
+      + econs 2; eauto.
+        { (* TODO: make lemma *) ii. eapply PTERM0. ii. eapply H5. ss. des; clarify. }
+        exploit L2wb; eauto.
+  }
 - (* continue step *)
-  inv H0. unfold E0 in H8; destruct H8; try congruence.
+  inv H0; cycle 1.
+  { destruct (Classical_Prop.classic (ev = Event_pterm)).
+    - clarify. right. split; ss. { unfold trace_intact. ii. apply H0. ss. eauto. } esplits; eauto.
+    - left. replace (trace_cut_pterm (ev :: t)) with (ev :: trace_cut_pterm (t)) in SRC; cycle 1.
+      { ss. des_ifs. }
+      apply star_non_E0_split' in SRC; ss. des_safe.
+      esplits; eauto. econs 2; eauto.
+      { (* TODO: make lemma *) ii. eapply PTERM. ii. eapply H3. ss. des; clarify. }
+  }
+  unfold E0 in H8; destruct H8; try congruence.
   exploit star_non_E0_split'; eauto. simpl. intros [s1x [P Q]].
+  left.
   exists i; exists s1x; split. left; auto. econstructor; eauto. simpl in H0; tauto.
+Unshelve.
+  all: eauto.
 Qed.
 
 Lemma fbs_progress:
@@ -1879,7 +1944,9 @@ Lemma fbs_progress:
   (exists r, final_state (atomic L2) s2 r) \/
   (exists t, exists s2', Step (atomic L2) s2 t s2').
 Proof.
-  intros. inv H. destruct t.
+  intros. inv H; cycle 1.
+  { destruct t; ss. { exfalso. (* TODO: make lemma *) eapply PTERM. ss. } right. esplits; eauto. econs; eauto. }
+  destruct t.
 - (* 1. no buffered events *)
   exploit (bsim_progress sim); eauto. eapply star_safe; eauto.
   intros [[r A] | [t [s2' A]]].
@@ -1915,7 +1982,9 @@ Proof.
   exists i; exists s1'; split. auto. econstructor. apply star_refl. auto. auto.
 - (* final states match *)
   intros. destruct s2 as [t s2]; simpl in H1; destruct H1; subst.
-  inv H. exploit (bsim_match_final_states sim); eauto. eapply star_safe; eauto.
+  inv H; cycle 1.
+  { exfalso. apply PTERM. ss. (* TODO: make lemma *) }
+  exploit (bsim_match_final_states sim); eauto. eapply star_safe; eauto.
   intros [s1'' [A B]]. exists s1''; split; auto. eapply star_trans; eauto.
 - (* progress *)
   eapply fbs_progress; eauto.
